Sinz amo proof

src/cardinality/sinz_amo.lean
@@ -12,8 +12,8 @@ import cnf.encoding
 import cnf.gensym
 
 import cardinality.distinct
-import cardinality.cardinality
-import cardinality.propagate
+import cardinality.amk
+import cardinality.alk
 
 import data.list.basic
 import data.nat.basic
@@ -22,6 +22,7 @@ variables {V : Type*} [inhabited V] [decidable_eq V]
 
 namespace sinz_amo
 
+open nat
 open list
 open literal
 open clause
@@ -30,11 +31,8 @@ open assignment
 open encoding
 open distinct
 open gensym
-open amo
-open propagate
-
--- NOTES: Proofs need to be cleaned up
---        Lemmas? The theorem length_lt_length_cons may be useful
+open amk
+open alk
 
 variables {l : list (literal V)} {lit l₁ l₂ : literal V} {g : gensym V}
           {τ : assignment V} (hdis : disjoint g.stock (clause.vars l))
@@ -62,7 +60,8 @@ begin
   exact set.not_mem_subset (fresh_stock_subset g) this
 end
 
--- NOTE: Only well-defined for lists with lengths ≥ 2
+-- A possible recursive definition. Proof was too challenging. Try again later?
+/-
 def sinz : Π (l : list (literal V)), Π (g : gensym V),
   (disjoint g.stock (clause.vars l)) → cnf V
 | []               _ _            := []
@@ -72,32 +71,401 @@ def sinz : Π (l : list (literal V)), Π (g : gensym V),
     [Neg g.fresh.1, Pos g.fresh.2.fresh.1] ::
     [Neg g.fresh.1, l₂.flip] ::
     (sinz (l₂ :: ls) g.fresh.2 (disjoint_fresh_of_disjoint hdis))
+-/
 
-def sinz2 : Π (l : list (literal V)), Π (g : gensym V),
-  (disjoint g.stock (clause.vars l)) → cnf V
-| [] _ _   := []
-| l g hdis := propagate ((g.nfresh (length l)).1.map Pos) ++
-    (l.take (length l - 1)).map_with_index (λ i x, [x.flip, Pos (g.nfresh i).2.fresh.1]) ++
-    (l.drop 1).map_with_index (λ i x, [Neg (g.nfresh i).2.fresh.1, x.flip])
+def xi_to_si (g : gensym V) (n i : nat) (lit : literal V) : cnf V :=
+  if (i < n - 1) then [[lit.flip, Pos (g.nth i)]] else []
 
-theorem enc : encodes amo (sinz2 l g hdis) l :=
+def si_to_next_si (g : gensym V) (n i : nat) : cnf V :=
+  if (i < n - 2) then [[Neg (g.nth i), Pos (g.nth (i + 1))]] else []
+
+def si_to_next_xi (g : gensym V) (i : nat) (lit : literal V) : cnf V :=
+  if (0 < i) then [[Neg (g.nth (i - 1)), lit.flip]] else []
+
+def sinz_amo (l : list (literal V)) (g : gensym V) : cnf V :=
+if hl : length l < 2 then [] else
+  join (map_with_index (λ (idx : nat) (lit : literal V),
+    xi_to_si g (length l) idx lit ++
+    si_to_next_si g (length l) idx ++
+    si_to_next_xi g idx lit) l)
+
+theorem xi_to_si_mem {l : list (literal V)} (hl : length l ≥ 2) (g : gensym V) 
+  {i : nat} (Hi' : i < length l - 1) (Hi : i < length l) :
+  [(l.nth_le i Hi).flip, Pos (g.nth i)] ∈ sinz_amo l g :=
 begin
-  intro τ,
+  rw sinz_amo,
+  simp [not_lt.mpr hl],
+  use (xi_to_si g l.length i (l.nth_le i Hi) ++ si_to_next_si g l.length i ++ si_to_next_xi g i (l.nth_le i Hi)),
   split,
-  {
-    intro hamo,
-    cases hamz : amz (map (literal.eval τ) l),
-    { rw ← amo.eval at hamo,
-      rw ← amz.eval at hamz,
-      rcases exists_eval_tt_of_eval_tt_of_amz_eval_ff hamo hamz with ⟨l₁, hmem, hl₁⟩,
-      
-    }
-  }
+  { use [l.nth_le i Hi, i, Hi],
+    simp only [eq_self_iff_true, append_assoc, and_self] },
+  { simp [xi_to_si, Hi'] }
 end
 
-#exit
+theorem si_to_next_si_mem {l : list (literal V)} (hl : length l ≥ 2) (g : gensym V)
+  {i : nat} (Hi' : i < length l - 2) (Hi : i < length l) :
+  [Neg (g.nth i), Pos (g.nth (i + 1))] ∈ sinz_amo l g :=
+begin
+  rw sinz_amo,
+  simp [not_lt.mpr hl],
+  use (xi_to_si g l.length i (l.nth_le i Hi) ++ si_to_next_si g l.length i ++ si_to_next_xi g i (l.nth_le i Hi)),
+  split,
+  { use [l.nth_le i Hi, i, Hi],
+    simp only [eq_self_iff_true, append_assoc, and_self] },
+  { simp [si_to_next_si, Hi'] }
+end
 
-theorem mem_sinz_vars_of_mem : length l ≥ 2 → clause.vars l ⊆ cnf.vars (sinz l g hdis) :=
+theorem si_to_next_xi_mem {l : list (literal V)} (hl : length l ≥ 2) (g : gensym V)
+  {i : nat} (Hi : 0 < i ∧ i < length l) :
+  [Neg (g.nth (i - 1)), (l.nth_le i Hi.2).flip] ∈ sinz_amo l g :=
+begin
+  rw sinz_amo,
+  simp [not_lt.mpr hl],
+  use (xi_to_si g l.length i (l.nth_le i Hi.2) ++ si_to_next_si g l.length i ++ si_to_next_xi g i (l.nth_le i Hi.2)),
+  split,
+  { use [l.nth_le i Hi.2, i, Hi.2],
+    simp only [eq_self_iff_true, append_assoc, and_self] },
+  { simp [si_to_next_xi, Hi.1] }
+end
+
+def nth_from_var (g : gensym V) (v : V) : nat → nat
+| 0       := 0
+| (i + 1) := if v = g.nth (i + 1) then i + 1 else nth_from_var i
+
+theorem nth_from_var_eq_nth_of_le (g : gensym V) {i n : nat} (Hi : i ≤ n) :
+  nth_from_var g (g.nth i) n = i :=
+begin
+  induction n with n ih generalizing i,
+  { cases i,
+    { refl },
+    { rw nonpos_iff_eq_zero at Hi,
+      exact absurd Hi (succ_ne_zero _) } },
+  { by_cases hn : i = n.succ,
+    { subst hn,
+      simp [nth_from_var] },
+    { simp [nth_from_var, nth_ne_of_ne hn],
+      exact ih (le_of_lt_succ (lt_of_le_of_ne Hi hn)) } }
+end
+
+def signal_truth (l : list (literal V)) (τ : assignment V) : nat → bool
+| 0       := l.head.eval τ
+| (i + 1) := if h : (i + 1) < length l then (l.nth_le (i + 1) h).eval τ || signal_truth i
+             else ff 
+
+def sinz_tau (l : list (literal V)) (g : gensym V) (τ : assignment V) : assignment V :=
+  λ v, if v ∈ clause.vars l then τ v else
+    signal_truth l τ (nth_from_var g v (length l))
+
+theorem signal_semantics {g : gensym V} {l : list (literal V)} 
+  (hdis : disjoint g.stock (clause.vars l)) {i : nat} :
+  i < length l → ∀ {τ : assignment V},
+  (signal_truth l τ i = tt ↔ alk.eval 1 τ (l.take (i + 1)) = tt) :=
+begin
+  intros hi τ,
+  induction i with i ih,
+  { simp [signal_truth, take_one_of_ne_nil (ne_nil_of_length_pos hi), 
+    alk.eval, alk, bool_symm] },
+  { simp [signal_truth, hi],
+    split,
+    { rintros (hs | hs),
+      { rw eval_take_tail_pos hi hs,
+        exact eval_zero _ _ },
+      { have ihred := (ih (lt_of_succ_lt hi)).mp hs,
+        have := take_sublist_of_le (le_succ (i + 1)) l,
+        exact eval_tt_of_sublist_of_eval_tt this ihred } },
+    { intro hl,
+      cases h : (l.nth_le (i + 1) _).eval τ,
+      { rw eval_take_tail_neg hi h at hl,
+        exact or.inr ((ih (lt_of_succ_lt hi)).mpr hl) },
+      { simp only [eq_self_iff_true, true_or] } } }
+end
+
+lemma minus_two {n m : nat} : n < m - 2 → n + 1 < m :=
+begin
+  intro h, cases m,
+  { linarith },
+  { cases m,
+    { linarith },
+    { simp only [succ_sub_succ_eq_sub, tsub_zero] at h,
+      exact lt_succ_of_lt (succ_lt_succ_iff.mpr h) } }
+end
+
+theorem xts_eval_tt {g : gensym V} {l : list (literal V)}
+  (hdis : disjoint g.stock (clause.vars l)) {i : nat} (Hi : i < length l) :
+  ∀ (τ : assignment V),
+  (xi_to_si g (length l) i (l.nth_le i Hi)).eval (sinz_tau l g τ) = tt :=
+begin
+  intro τ,
+  rw eval_tt_iff_forall_clause_eval_tt,
+  intros c hc,
+  rw [xi_to_si] at hc,
+  by_cases Hi₂ : (i = l.length - 1),
+  { simp [Hi₂] at hc, contradiction },
+  { simp [lt_of_le_of_ne (le_pred_of_lt Hi) Hi₂] at hc,
+    subst hc,
+    rw eval_tt_iff_exists_literal_eval_tt,
+    cases hl : (l.nth_le i Hi).eval τ,
+    { use (l.nth_le i Hi).flip,
+      have hmem := mem_vars_of_mem (nth_le_mem l i Hi),
+      cases l.nth_le i Hi;
+      { rw var at hmem,
+        rw literal.eval at hl,
+        simp [eval_flip, literal.eval, hl, sinz_tau, hmem] } },
+    { use Pos (g.nth i),
+      simp [literal.eval, sinz_tau, forall_nth_not_mem_of_disjoint' hdis i,
+        nth_from_var_eq_nth_of_le g (le_of_lt Hi)],
+      cases i,
+      { rw signal_truth, rw nth_le_zero at hl, exact hl },
+      { simp [signal_truth, Hi], exact or.inl hl } } }
+end
+
+theorem stns_eval_tt {g : gensym V} {l : list (literal V)}
+  (hdis : disjoint g.stock (clause.vars l)) :
+  ∀ (i : nat) (τ : assignment V),
+  (si_to_next_si g (length l) i).eval (sinz_tau l g τ) = tt :=
+begin
+  intros i τ,
+  rw eval_tt_iff_forall_clause_eval_tt,
+  intros c hc,
+  rw si_to_next_si at hc,
+  by_cases hi : (i < l.length - 2),
+  { simp [hi] at hc,
+    subst hc,
+    rw eval_tt_iff_exists_literal_eval_tt,
+    cases hs : (sinz_tau l g τ) (g.nth i),
+    { use Neg (g.nth i),
+      simp [literal.eval, hs] },
+    { use Pos (g.nth (i + 1)),
+      simp [literal.eval, sinz_tau, forall_nth_not_mem_of_disjoint' hdis (i + 1)],
+      have : i + 1 < l.length, from minus_two hi,
+      rw nth_from_var_eq_nth_of_le g (le_of_lt this),
+      simp [signal_truth, this],
+      simp [sinz_tau, forall_nth_not_mem_of_disjoint' hdis i,
+        nth_from_var_eq_nth_of_le g (le_of_lt (lt_of_succ_lt this))] at hs,
+      exact or.inr hs } },
+  { simp [hi] at hc, contradiction }
+end
+
+theorem stnx_eval_tt {g : gensym V} {l : list (literal V)}
+  (hdis : disjoint g.stock (clause.vars l)) {i : nat} (Hi : i < length l) :
+  ∀ (τ : assignment V), amk.eval 1 τ (l.take (i + 1)) = tt →
+  (si_to_next_xi g i (l.nth_le i Hi)).eval (sinz_tau l g τ) = tt :=
+begin
+  intros τ hamo,
+  rw eval_tt_iff_forall_clause_eval_tt,
+  intros c hc,
+  rw si_to_next_xi at hc,
+  cases i; simp at hc,
+  { contradiction },
+  { subst hc,
+    rw eval_tt_iff_exists_literal_eval_tt,
+    cases hs : (sinz_tau l g τ) (g.nth i),
+    { use Neg (g.nth i),
+      simp [hs, literal.eval] },
+    { simp [sinz_tau, forall_nth_not_mem_of_disjoint' hdis i] at hs,
+      rw nth_from_var_eq_nth_of_le g (le_of_lt (lt_of_succ_lt Hi)) at hs,
+      cases ht : (l.nth_le _ Hi).eval (sinz_tau l g τ),
+      { use (l.nth_le _ Hi).flip,
+        simp [eval_flip, literal.eval, ht] },
+      { have heqod : eqod (sinz_tau l g τ) τ (clause.vars l),
+        { rw sinz_tau,
+          intros v hv,
+          simp [hv] },
+        have := (signal_semantics hdis (lt_of_succ_lt Hi)).mp hs,
+        have hmem := mem_vars_of_mem (nth_le_mem l _ Hi),
+        rw eval_eq_of_eqod_of_var_mem heqod hmem at ht,
+        rw eval_tail_pos ht at hamo,
+        rw alk_of_amk_of_gt hamo nat.one_pos at this,
+        contradiction } } }
+end
+
+-- Forward direction
+theorem sinz_forward {τ : assignment V} {l : list (literal V)} {g : gensym V} 
+  (hdis : disjoint g.stock (clause.vars l)) :
+  amk.eval 1 τ l = tt → (sinz_amo l g).eval (sinz_tau l g τ) = tt :=
+begin
+  intro hamo,
+  rw eval_tt_iff_forall_clause_eval_tt,
+  intros c hc,
+  by_cases hl : length l < 2,
+  { simp [sinz_amo, hl] at hc, exfalso, exact hc },
+  { simp [sinz_amo, hl] at hc,
+    rcases hc with ⟨f, ⟨lit, i, ⟨Hi, rfl⟩, rfl⟩, hc⟩,
+    simp at hc,
+    rcases hc with (hc | hc | hc),
+    { have := xts_eval_tt hdis Hi τ,
+      exact eval_tt_iff_forall_clause_eval_tt.mp this _ hc },
+    { have := stns_eval_tt hdis i τ,
+      exact eval_tt_iff_forall_clause_eval_tt.mp this _ hc },
+    { have := amk.eval_take hamo (i + 1),
+      have := stnx_eval_tt hdis Hi τ this,
+      rw si_to_next_xi at hc,
+      by_cases hiz : (0 < i),
+      { simp [hiz] at hc, subst hc,
+        simp [si_to_next_xi, eval_tt_iff_forall_clause_eval_tt, hiz] at this,
+        exact this },
+      { simp [hiz] at hc, exfalso, exact hc } } } 
+end
+
+-- Reverse direction --
+
+-- Proofs for necessary conditions for setting signal variables to true
+theorem signal_nec2 {τ} {l : list (literal V)} (hl : length l ≥ 2) {g : gensym V} 
+  {i : nat} (hi : i < length l - 2) :
+  (sinz_amo l g).eval τ = tt →
+  τ (g.nth i) = tt → ∀ {j : nat}, (j > i ∧ j < length l - 1) → τ (g.nth j) = tt :=
+begin
+  rintros hs hg j ⟨hij, hj⟩,
+  induction j with j ih,
+  { linarith },
+  { by_cases hij' : i = j,
+    { subst hij',
+      have := si_to_next_si_mem hl g hi (lt_of_succ_lt (minus_two hi)),
+      have := eval_tt_iff_forall_clause_eval_tt.mp hs _ (this),
+      simp [eval_tt_iff_exists_literal_eval_tt] at this,
+      rcases this with ⟨lit, (rfl | rfl), hlit⟩,
+      { simp [literal.eval, hg] at hlit, contradiction },
+      { rw literal.eval at hlit, exact hlit } },
+    { have := lt_of_le_of_ne (le_of_lt_succ hij) hij',
+      have ihred := ih this (lt_of_succ_lt hj),
+      have hjl : j < length l,
+      { rcases exists_eq_add_of_le hl with ⟨k, hk⟩,
+        rw add_comm at hk,
+        simp [hk] at hj |-,
+        exact lt_of_succ_lt (lt_succ_of_lt hj) },
+      have : j < length l - 2,
+      { rcases exists_eq_add_of_le hl with ⟨k, hk⟩,
+        rw add_comm at hk,
+        simp [hk] at hj |-,
+        exact succ_lt_succ_iff.mp hj },
+      have := si_to_next_si_mem hl g this hjl,
+      have := eval_tt_iff_forall_clause_eval_tt.mp hs _ this,
+      simp [eval_tt_iff_exists_literal_eval_tt] at this,
+      rcases this with ⟨list, (rfl | rfl), hlit⟩,
+      { simp [literal.eval, ihred] at hlit, contradiction },
+      { rw literal.eval at hlit, exact hlit } } }
+end
+
+theorem signal_nec {τ} {l : list (literal V)} (hl : length l ≥ 2) {g : gensym V}
+  {i : nat} (hi : i < length l - 1) :
+  (sinz_amo l g).eval τ = tt → 
+  alk.eval 1 τ (l.take (i + 1)) = tt → τ (g.nth i) = tt :=
+begin
+  intros hs hlk,
+  induction i with i ih,
+  { cases l with l ls,
+    { rw length at hi, linarith },
+    { rw length at hl,
+      have : ls.length > 0, linarith,
+      have : [l.flip, Pos (g.nth 0)] ∈ ite (0 < ls.length) [[l.flip, Pos (g.nth 0)]] [],
+      { have : 0 < ls.length, exact this,
+        simp [this] },
+      simp [alk.eval, alk] at hlk,
+      simp [sinz_amo, not_lt.mpr hl, eval_tt_iff_forall_clause_eval_tt, xi_to_si] at hs,
+      have := hs _ (or.inl this),
+      simp [eval_tt_iff_exists_literal_eval_tt] at this,
+      rcases this with ⟨lit, (rfl | rfl), hlit⟩,
+      { rw [eval_flip, ← hlk] at hlit, contradiction },
+      { rw literal.eval at hlit, exact hlit } } },
+  { have : i + 1 < length l, from lt_of_lt_pred hi,
+    cases hx : literal.eval τ (l.nth_le _ this),
+    { rw eval_take_tail_neg this hx at hlk,
+      have ihred := ih (lt_of_succ_lt hi) hlk,
+      -- Apply signal_nec2
+      have : i < l.length - 2,
+      { rcases exists_eq_add_of_le hl with ⟨k, hk⟩,
+        rw add_comm at hk,
+        simp [hk] at hi |-,
+        exact succ_lt_succ_iff.mp hi },
+      apply signal_nec2 hl this hs ihred,
+      split,
+      { exact lt_succ_self i },
+      { rcases exists_eq_add_of_le hl with ⟨k, hk⟩,
+        rw add_comm at hk,
+        simp [hk] at this |-,
+        exact succ_lt_succ_iff.mpr this } },
+    { have hmem := xi_to_si_mem hl g hi this,
+      have := eval_tt_iff_forall_clause_eval_tt.mp hs _ hmem,
+      simp [eval_tt_iff_exists_literal_eval_tt] at this,
+      rcases this with ⟨list, (rfl | rfl), hlit⟩,
+      { rw [eval_flip, hx] at hlit, contradiction },
+      { rw literal.eval at hlit, exact hlit } } }
+end
+
+theorem signal_nec3 {τ} {l : list (literal V)} (hl : length l ≥ 2) {g : gensym V}
+  {i : nat} (hi : i < length l) :
+  (sinz_amo l g).eval τ = tt → τ (g.nth i) = tt → 
+  ∀ {j : nat} (hj : (j > i ∧ j < length l)), (l.nth_le j hj.2).eval τ = ff :=
+begin
+  rintros hs hg j ⟨hij, hj⟩,
+  have hs' := hs,
+  rw eval_tt_iff_forall_clause_eval_tt at hs,
+  have hc := hs _ (si_to_next_xi_mem hl g ⟨pos_of_gt hij, hj⟩),
+  by_cases hj' : (j - 1) = i,
+  { rw [hj', eval_tt_iff_exists_literal_eval_tt] at hc,
+    simp at hc,
+    rcases hc with ⟨lit, (rfl | rfl), he⟩,
+    { simp [literal.eval, hg] at he, contradiction },
+    { simp [eval_flip] at he, exact he } },
+  { have hsub : j - 1 > i,
+    { have := pos_of_gt hij,
+      cases j,
+      { linarith },
+      { have : i ≤ j, exact lt_succ_iff.mp hij,
+        simp at hj' |-,
+        exact lt_of_le_of_ne this (ne.symm hj') } },
+    have : j - 1 < length l - 1,
+    { rcases exists_eq_add_of_le hl with ⟨k, hk⟩,
+      rw add_comm at hk,
+      simp [hk] at hj |-,
+      cases j,
+      { simp },
+      { simp, exact succ_lt_succ_iff.mp hj } },
+    have hi₂ : i < l.length - 2,
+    { rcases exists_eq_add_of_le hl with ⟨k, hk⟩,
+      rw add_comm at hk,
+      simp [hk] at this |-,
+      exact lt_of_lt_of_le hsub (le_of_lt_succ this) },
+    have := signal_nec2 hl hi₂ hs' hg ⟨hsub, this⟩,
+    simp [eval_tt_iff_exists_literal_eval_tt] at hc,
+    rcases hc with ⟨lit, (rfl | rfl), he⟩,
+    { simp [literal.eval, this] at he, contradiction },
+    { simp [eval_flip] at he, exact he } }
+end
+
+theorem sinz_reverse {τ} {l : list (literal V)} {g : gensym V}
+  (hdis : disjoint g.stock (clause.vars l)) :
+  (sinz_amo l g).eval τ = tt → amk.eval 1 τ l = tt :=
+begin
+  intro hs,
+  by_cases hl : length l ≥ 2,
+  { rw amo_eval_tt_iff_distinct_eval_ff_of_eval_tt,
+    rintros lit₁ lit₂ ⟨i, j, hi, hj, hij, rfl, rfl⟩ hl₁,
+    have : i < length l - 1, from lt_of_lt_of_le hij (le_pred_of_lt hj),
+    have := signal_nec hl this hs (amo_take_of_tt hi hl₁),
+    exact signal_nec3 hl hi hs this ⟨hij, hj⟩ },
+  { rw not_le at hl,
+    exact eval_tt_of_ge_length (le_of_lt_succ hl) _ }
+end
+
+theorem sinz_amo_encodes_amo {l : list (literal V)} {g : gensym V} 
+  (hdis : disjoint g.stock (clause.vars l)) : 
+  encodes (amk 1) (sinz_amo l g) l :=
+begin
+  intro τ, split,
+  { intro hamo,
+    use sinz_tau l g τ,
+    split,
+    { exact sinz_forward hdis hamo },
+    { intros v hv, simp [sinz_tau, hv] } },
+  { rintros ⟨σ, hs, heqod⟩,
+    rw [← amk.eval, eval_eq_amk_of_eqod 1 heqod],
+    exact sinz_reverse hdis hs }
+end
+
+/-
+theorem mem_sinz_vars_of_mem {l : list (literal V)} {g : gensym V} : 
+  length l ≥ 2 → clause.vars l ⊆ cnf.vars (sinz_amo l g hdis) :=
 begin
   intro hlen,
   induction l using strong_induction_on_lists with l ih generalizing g,
@@ -179,559 +547,6 @@ begin
     rcases hvar with ⟨hvar₁, hvar₂, hvar₃, hvar⟩,
     simp [cnf.vars, clause.vars, not_or_distrib, flip_var_eq, var,
       hvar₁, hvar₂, hvar₃, hg₁, hg₂, ihred] }
-end
-
-/-
-theorem sinz_amz : amz.eval τ l = tt → 
-  (sinz l g hdis).eval (assignment.ite (clause.vars l) τ all_ff) = tt :=
-begin
-  induction l using strong_induction_on_lists with l ih generalizing g,
-  cases l with l₁ ls,
-  { simp [sinz] },
-  { cases ls with l₂ ls,
-    { simp [sinz] },
-    { intro hamz,
-      have hdis' := disjoint_fresh_of_disjoint hdis,
-      rw [eval_tt_iff_forall_clause_eval_tt, sinz],
-      intros c hc,
-      simp at hc,
-      rw eval_tt_iff_exists_literal_eval_tt,
-      rcases hc with (rfl | rfl | rfl | hc),
-      { use l₁.flip,
-        rw [eval_flip,ite_pos_lit (mem_vars_of_mem (mem_cons_self l₁ _))],
-        rw amz.eval_tt_iff_forall_eval_ff at hamz,
-        simp [hamz l₁ (mem_cons_self l₁ _)] },
-      { use Neg g.fresh.1,
-        have := set.disjoint_left.mp hdis (fresh_mem_stock g), -- TODO why not ellide?
-        simp [literal.eval, ite_neg this, all_ff] },
-      { use Neg g.fresh.1,
-        have := set.disjoint_left.mp hdis (fresh_mem_stock g), -- TODO why not ellide?
-        simp [literal.eval, ite_neg this, all_ff] },
-      { have hlen : length (l₂ :: ls) < length (l₁ :: l₂ :: ls), simp,
-        have := ih (l₂ :: ls) hlen hdis' (amz.eval_tt_of_eval_tt_cons hamz),
-        rw eval_tt_iff_forall_clause_eval_tt at this,
-        rcases eval_tt_iff_exists_literal_eval_tt.mp (this c hc) with ⟨l, hlc, hl⟩,
-        use [l, hlc],
-        by_cases hlmem : (l.var ∈ clause.vars (l₂ :: ls)),
-        { rw ite_pos_lit (vars_subset_of_vars_cons l₁ (l₂ :: ls) hlmem),
-          rw ite_pos_lit hlmem at hl,
-          exact hl },
-        { rw ite_neg_lit hlmem at hl,
-          by_cases h₁ : l₁.var ∈ clause.vars (l₂ :: ls),
-          { have : l.var ∉ clause.vars (l₁ :: l₂ :: ls),
-            { rw clause.vars,
-              intro hcon,
-              rcases finset.mem_union.mp hcon with (hcon | hcon),
-              { simp at hcon,
-                rw ← hcon at h₁,
-                exact hlmem h₁ },
-              { exact hlmem hcon } },
-            rw ite_neg_lit this,
-            exact hl },
-          { have := mem_vars_of_mem (mem_cons_self l₁ (l₂ :: ls)),
-            have := set.disjoint_right.mp hdis this,
-            have := set.not_mem_subset (fresh_stock_subset g) this,
-            have h₁' := not_mem_sinz_vars_of_not_mems hdis' h₁ this,
-            have := clause_vars_subset_of_vars_of_mem hc
-              (mem_vars_of_mem hlc),
-            --have : l.var ≠ l₁.var, library_search,
-            have := ne_of_mem_of_not_mem this h₁',
-            have : l.var ∉ clause.vars (l₁ :: l₂ :: ls),
-            { rw clause.vars,
-              simp [not_or_distrib],
-              exact ⟨this, hlmem⟩ },
-            rw ite_neg_lit this,
-            exact hl } } } } }
-end
--/
-
--- NOTE: This theorem and the above are very similar, fixes to one go to other
-theorem sinz_amz' : amz.eval τ l = tt →
-  (sinz l g hdis).eval (assignment.ite (clause.vars l) τ all_tt) = tt :=
-begin
-  induction l using strong_induction_on_lists with l ih generalizing g,
-  cases l with l₁ ls,
-  { simp [sinz] },
-  { cases ls with l₂ ls,
-    { simp [sinz] },
-    { intro hamz,
-      have hdis' := disjoint_fresh_of_disjoint hdis,
-      rw [eval_tt_iff_forall_clause_eval_tt, sinz],
-      intros c hc,
-      simp at hc,
-      rw eval_tt_iff_exists_literal_eval_tt,
-      rcases hc with (rfl | rfl | rfl | hc),
-      { use l₁.flip,
-        rw [eval_flip, ite_pos_lit (mem_vars_of_mem (mem_cons_self l₁ _))],
-        rw amz.eval_tt_iff_forall_eval_ff at hamz,
-        simp [hamz l₁ (mem_cons_self l₁ _)] },
-      { use Pos g.fresh.2.fresh.1,
-        have := set.disjoint_left.mp hdis (fresh_fresh_mem_stock g),
-        simp [literal.eval, ite_neg this, all_tt] },
-      { use l₂.flip,
-        have : l₂.var ∈ clause.vars (l₁ :: l₂ :: ls), simp [clause.vars],
-        rw [eval_flip, ite_pos_lit this],
-        rw amz.eval_tt_iff_forall_eval_ff at hamz,
-        simp [hamz l₂ (mem_cons_of_mem _ (mem_cons_self l₂ _))] },
-      { have hlen : length (l₂ :: ls) < length (l₁ :: l₂ :: ls), simp,
-        have := ih (l₂ :: ls) hlen hdis' (amz.eval_tt_of_eval_tt_cons hamz),
-        rw eval_tt_iff_forall_clause_eval_tt at this,
-        rcases eval_tt_iff_exists_literal_eval_tt.mp (this c hc) with ⟨l, hlc, hl⟩,
-        use [l, hlc],
-        by_cases hlmem : (l.var ∈ clause.vars (l₂ :: ls)),
-        { rw ite_pos_lit (vars_subset_of_vars_cons l₁ (l₂ :: ls) hlmem),
-          rw ite_pos_lit hlmem at hl,
-          exact hl },
-        { rw ite_neg_lit hlmem at hl,
-          by_cases h₁ : l₁.var ∈ clause.vars (l₂ :: ls),
-          { have : l.var ∉ clause.vars (l₁ :: l₂ :: ls),
-            { rw clause.vars,
-              intro hcon,
-              rcases finset.mem_union.mp hcon with (hcon | hcon),
-              { simp at hcon,
-                rw ← hcon at h₁,
-                exact hlmem h₁ },
-              { exact hlmem hcon } },
-            rw ite_neg_lit this,
-            exact hl },
-          { have := mem_vars_of_mem (mem_cons_self l₁ (l₂ :: ls)),
-            have := set.disjoint_right.mp hdis this,
-            have := set.not_mem_subset (fresh_stock_subset g) this,
-            have h₁' := not_mem_sinz_vars_of_not_mems hdis' h₁ this,
-            have := clause_vars_subset_of_vars_of_mem hc
-              (mem_vars_of_mem hlc),
-            --have : l.var ≠ l₁.var, library_search,
-            have := ne_of_mem_of_not_mem this h₁',
-            have : l.var ∉ clause.vars (l₁ :: l₂ :: ls),
-            { rw clause.vars,
-              simp [not_or_distrib],
-              exact ⟨this, hlmem⟩ },
-            rw ite_neg_lit this,
-            exact hl } } } } }
-end
-
-theorem sinz_amo (hdis : disjoint g.stock (clause.vars (l₁ :: l))) : 
-  amz.eval τ l = tt → l₁.eval τ = tt → 
-  (sinz (l₁ :: l) g hdis).eval (assignment.ite (clause.vars (l₁ :: l)) τ all_tt) = tt :=
-begin
-  intros hamz h₁,
-  cases l with l₂ ls,
-  { simp [sinz] },
-  { rw [eval_tt_iff_forall_clause_eval_tt, sinz],
-    intros c hc,
-    simp at hc,
-    rw eval_tt_iff_exists_literal_eval_tt,
-    rcases hc with (rfl | rfl | rfl | hc),
-    { use Pos g.fresh.1,
-      have := set.disjoint_left.mp hdis (fresh_mem_stock g),
-      simp [literal.eval, ite_neg this, all_tt] },
-    { use Pos g.fresh.2.fresh.1,
-      have := set.disjoint_left.mp hdis (fresh_fresh_mem_stock g),
-      simp [literal.eval, ite_neg this, all_tt] },
-    { use l₂.flip,
-      have : l₂.var ∈ clause.vars (l₁ :: l₂ :: ls), simp [clause.vars],
-      rw [eval_flip, ite_pos_lit this],
-      rw amz.eval_tt_iff_forall_eval_ff at hamz,
-      simp [hamz l₂ (mem_cons_self l₂ _)] },
-    {
-      have hdis' := disjoint_fresh_of_disjoint hdis,
-      have := sinz_amz' hdis' hamz,
-      rw eval_tt_iff_forall_clause_eval_tt at this,
-      rcases eval_tt_iff_exists_literal_eval_tt.mp (this c hc) with ⟨l, hlc, hl⟩,
-      use [l, hlc],
-      have := cnf.clause_vars_subset_of_vars_of_mem hc,
-      rcases mem_or_mem_of_mem_vars hdis' (this (mem_vars_of_mem hlc)) with (hv | hv),
-      { rw ite_pos_lit (mem_vars_cons_of_mem_vars l₁ hv),
-        rw ite_pos_lit hv at hl,
-        exact hl },
-      { have := set.disjoint_left.mp hdis (fresh_stock_subset g hv),
-        rw ite_neg_lit this,
-        rw clause.vars at this,
-        simp [not_or_distrib] at this,
-        rw ite_neg_lit this.2 at hl,
-        exact hl } } }
-end
-
-theorem sinz_signal (hdis : disjoint g.stock (clause.vars (l₁ :: l))) :
-  τ g.fresh.1 = tt → (sinz (l₁ :: l) g hdis).eval τ = tt → 
-  ∀ (lit : literal V), lit ∈ l → lit.eval τ = ff :=
-begin
-  sorry,
-  /-
-  intro ht,
-  induction l using strong_induction_on_lists with l ih generalizing g,
-  cases l with l₂ ls,
-  { simp [sinz] },
-  intros heval lit hlit,
-  rw [sinz, eval_tt_iff_forall_clause_eval_tt] at heval,
-  simp at heval,
-  rcases heval with ⟨h₁, h₂, h₃, h₄⟩,
-  have hlen : length ls < length (l₂ :: ls), simp,
-  have hdis' : disjoint g.fresh.2.stock (clause.vars (l₁ :: ls)),
-  {
-    apply set.disjoint_right.mpr,
-    intros v hv,
-    have : clause.vars (l₁ :: ls) ⊆ clause.vars (l₁ :: l₂ :: ls),
-    { apply clause.vars_subset_of_subset,
-      simp [subset_cons_of_subset l₁ (subset_cons l₂ ls)] },
-    have := this hv,
-    have := set.disjoint_right.mp hdis this,
-    intro hcon,
-    exact this (fresh_stock_subset g hcon) },
-    have ihred := ih _ hlen hdis',
-    sorry
-
-   simp [sinz, eval_tt_iff_forall_clause_eval_tt],
-    rintros ht hc₁ hc₂ hc₃ rfl,
-    simp [eval_tt_iff_exists_literal_eval_tt] at hc₃,
-    rcases hc₃ with ⟨l, (rfl | rfl), hl⟩,
-    { rw [literal.eval, ht] at hl, contradiction },
-    { simp [eval_flip] at hl, exact hl } },
-  {
-    intros ht heval,
-    rw [sinz, eval_tt_iff_forall_clause_eval_tt] at heval,
-    simp at heval,
-    have hlen : length (l₃ :: ls) < length (l₂ :: l₃ :: ls), simp,
-    have hdis' := disjoint_fresh_of_disjoint hdis,
-    have ihred := (ih _ hlen hdis'),
-
-  }
-  -/
-end
-
-#exit
-
-theorem sinz_base_case (hdis : disjoint g.stock (clause.vars [l₁, l₂])) : 
-  encodes amo (sinz [l₁, l₂] g hdis) [l₁, l₂] :=
-begin
-  intro τ,
-  split,
-  { intro hamo,
-    cases h₁ : (literal.eval τ l₁),
-    { use assignment.ite (clause.vars [l₁, l₂]) τ all_ff,
-      split,
-      { have hnmem₁ : g.fresh.1 ∉ clause.vars [l₁, l₂],
-        { have := set.disjoint_left.mp hdis (fresh_mem_stock g), assumption },
-        rw eval_tt_iff_forall_clause_eval_tt,
-        intros c hc,
-        simp [sinz] at hc,
-        rw eval_tt_iff_exists_literal_eval_tt,
-        rcases hc with (rfl | rfl | rfl),
-        { use l₁.flip,
-          have hmem₁ : l₁.flip.var ∈ clause.vars [l₁, l₂],
-          { simp [flip_var_eq, clause.vars] },
-          rw [ite_pos_lit hmem₁, eval_flip],
-          simp [h₁] },
-        { use Neg g.fresh.1,
-          simp [literal.eval, ite_neg hnmem₁, all_ff] },
-        { use Neg g.fresh.1,
-          simp [literal.eval, ite_neg hnmem₁, all_ff]
-        } },
-      { exact (ite_eqod _ _ _).symm } },
-    { rw [← amo.eval, eval_cons_pos h₁] at hamo,
-      use [(assignment.ite (clause.vars [l₁, l₂]) τ all_tt),
-        sinz_amo hdis hamo h₁, (ite_eqod _ _ _).symm] } },
-  { rintros ⟨σ, heval, heqod⟩,
-    have heq : literal.eval τ l₂ = literal.eval σ l₂,
-    { have : l₂.var ∈ clause.vars [l₁, l₂],
-      { simp [clause.vars] },
-        exact eval_eq_of_eqod_of_var_mem heqod this },
-      rw [← amo.eval, eval_eq_amo_of_eqod heqod],
-      rw eval_tt_iff_forall_clause_eval_tt at heval,
-      cases h₁ : (literal.eval σ l₁),
-      { rw [eval_cons_neg h₁, amo.eval_singleton] },
-      { have : ∀ (lit₁ lit₂ : literal V), (distinct lit₁ lit₂ [l₁, l₂]) → 
-          lit₁.eval τ = tt → lit₂.eval τ = ff,
-        { intros lit₁ lit₂ hd _,
-          rcases eq_of_distinct_double hd with ⟨rfl, rfl⟩,
-          simp [sinz, clause.eval, eval_flip, literal.eval, h₁] at heval,
-          rcases heval with ⟨hs₁, hs₂, hs₃⟩,
-          simp [hs₁] at hs₃,
-          rw heq,
-          exact hs₃ },
-        rw ← eval_eq_amo_of_eqod heqod,
-        exact amo_eval_tt_iff_distinct_eval_ff_of_eval_tt.mpr this } }
-end
-
-theorem sinz_encodes_amo : encodes amo (sinz l g hdis) l :=
-begin
-  induction l using strong_induction_on_lists with l ih generalizing g,
-  cases l with l₁ ls,
-  { intro τ, simp [sinz] },
-  cases ls with l₂ ls,
-  { intro τ, simp [sinz], use τ },
-
-  have hdis' := disjoint_fresh_of_disjoint hdis,
-
-  cases ls with l₃ ls,
-  { exact sinz_base_case hdis },
-  { intro τ, 
-    have hlen : length (l₂ :: l₃ :: ls) < length (l₁ :: l₂ :: l₃ :: ls), simp,
-    have ihred := (ih _ hlen hdis') τ,
-    split,
-    { intro hamo,
-      cases h₁ : (literal.eval τ l₁),
-      { rcases ihred.mp (eval_tt_of_eval_tt_cons hamo) with ⟨σ, heval', hs⟩,
-        use assignment.ite (cnf.vars (sinz (l₂ :: l₃ :: ls) g.fresh.2 hdis')) σ 
-            (assignment.ite {l₁.var} τ all_ff),
-        have heval₁ : literal.eval (assignment.ite (cnf.vars (sinz (l₂ :: l₃ :: ls) g.fresh.2 hdis')) σ 
-            (assignment.ite {l₁.var} τ all_ff)) l₁ = ff,
-        { by_cases h : (l₁.var ∈ cnf.vars (sinz (l₂ :: l₃ :: ls) g.fresh.2 hdis')),
-          { rw ite_pos_lit h,
-            rcases mem_or_mem_of_mem_vars hdis' h with (hv | hv),
-            { rw ← eval_eq_of_eqod_of_var_mem hs hv,
-              exact h₁ },
-            { have : l₁.var ∈ clause.vars (l₁ :: l₂ :: l₃ :: ls),
-              { rw clause.vars,
-                exact finset.mem_union.mpr (or.inl (finset.mem_singleton_self l₁.var)) },
-              have := set.disjoint_right.mp hdis this,
-              have := (fresh_stock_subset g) hv,
-              contradiction } },
-          { rw ite_neg_lit h,
-            rw ite_pos_lit (finset.mem_singleton_self l₁.var),
-            exact h₁ } },
-        have heval₂ : (assignment.ite (cnf.vars (sinz (l₂ :: l₃ :: ls) g.fresh.2 hdis')) σ 
-            (assignment.ite {l₁.var} τ all_ff)) g.fresh.1 = ff,
-        { 
-          have h₀ := set.disjoint_left.mp hdis (fresh_mem_stock g),
-          have h₁ : g.fresh.1 ∉ clause.vars (l₂ :: l₃ :: ls),
-          { rw clause.vars at h₀,
-            simp [not_or_distrib] at h₀,
-            exact h₀.2 },
-          have h₂ : g.fresh.1 ∉ g.fresh.2.stock,
-          { exact fresh_not_mem_fresh_stock g },
-          rw ite_neg (not_mem_sinz_vars_of_not_mems hdis' h₁ h₂),
-          rw clause.vars at h₀,
-          simp [not_or_distrib] at h₀,
-          have : g.fresh.1 ∉ {l₁.var},
-          { rw finset.mem_singleton,
-            exact h₀.1 },
-          rw [ite_neg this, all_ff] },
-        split,
-        { rw [eval_tt_iff_forall_clause_eval_tt, sinz],
-          intros c hc,
-          rw eval_tt_iff_exists_literal_eval_tt,
-          simp at hc,
-          rcases hc with (rfl | rfl | rfl | hc),
-          { use l₁.flip,
-            simp [eval_flip, heval₁] },
-          { use Neg g.fresh.1,
-            simp [literal.eval, heval₂] },
-          { use Neg g.fresh.1,
-            simp [literal.eval, heval₂] },
-          { rw ← eval_tt_iff_exists_literal_eval_tt,
-            rw eval_tt_iff_forall_clause_eval_tt at heval',
-            rw ← heval' c hc,
-            apply eval_eq_clause_of_eqod,
-            apply eqod_subset (clause_vars_subset_of_vars_of_mem hc),
-            intros v hv,
-            rw ite_pos hv } },
-        { intros v hv,
-          rcases finset.mem_union.mp hv with (hvmem | hvmem),
-          { cases l₁;
-            { simp [literal.flip, literal.eval, var] at h₁ hvmem heval₁ |-,
-              simp [heval₁, hvmem, h₁] } },
-          { have : length (l₂ :: l₃ :: ls) ≥ 2, dec_trivial,
-            rw ite_pos (mem_sinz_vars_of_mem hdis' this hvmem),
-            exact hs v hvmem } } },
-      { rw [← amo.eval, eval_cons_pos h₁] at hamo,
-        use [(assignment.ite (clause.vars (l₁ :: l₂ :: l₃ :: ls)) τ all_tt),
-        sinz_amo hdis hamo h₁, 
-        (ite_eqod (clause.vars (l₁ :: l₂ :: l₃ :: ls)) τ _).symm] } },
-    { rintros ⟨σ, heval, heqod⟩,
-      cases h₁ : (literal.eval τ l₁),
-      { rw [eval_tt_iff_forall_clause_eval_tt, sinz] at heval,
-        simp at heval,
-        rcases heval with ⟨hc₁, hc₂, hc₃, hc₄⟩,
-        rw ← eval_tt_iff_forall_clause_eval_tt at hc₄,
-        rw [← amo.eval, eval_cons_neg h₁],
-        exact ihred.mpr ⟨σ, hc₄, eqod_subset (vars_subset_of_vars_cons _ _) heqod⟩ },
-      { rw [← amo.eval, eval_cons_pos h₁],
-        cases hf : (σ g.fresh.1),
-        { rw [eval_tt_iff_forall_clause_eval_tt] at heval,
-          have : [l₁.flip, Pos (g.fresh.1)] ∈ sinz (l₁ :: l₂ :: l₃ :: ls) g hdis,
-          { exact mem_cons_self _ _ },
-          have := heval _ this,
-          simp [eval_tt_iff_exists_literal_eval_tt] at this,
-          rcases this with ⟨w, (rfl | rfl), hw⟩,
-          { rw [eval_flip, ← h₁] at hw, -- This can be cleaned up
-            have := eval_eq_of_eqod_of_var_mem heqod (mem_vars_of_mem (mem_cons_self l₁ _)),
-            rw h₁ at this,
-            simp [← this] at hw,
-            rw ← hw at h₁,
-            contradiction },
-          { rw [literal.eval, hf] at hw,
-            contradiction } },
-        { rw amz.eval_eq_amz_of_eqod (eqod_subset (vars_subset_of_vars_cons l₁ (l₂ :: l₃ :: ls)) heqod),
-          exact amz.eval_tt_iff_forall_eval_ff.mpr (sinz_signal hdis hf heval) } } } }
-end
-
-/-
-theorem sinz_encodes_amo : length l ≥ 2 → encodes amo (sinz l g hdis) l :=
-begin
-  intros hl τ,
-  induction l using strong_induction_on_lists with l ih generalizing g,
-  rcases exists_cons_cons_of_length_ge_two hl with ⟨l₁, l₂, ls, rfl⟩,
-  have hdis' := disjoint_fresh_of_disjoint hdis,
-  have hmem₁ : l₁.flip.var ∈ clause.vars (l₁ :: l₂ :: ls),
-  { simp [flip_var_eq, clause.vars] },
-  have hmemnot₁ : l₁.flip.var ∉ g.stock,
-  { exact set.disjoint_right.mp hdis hmem₁ },
-  have hmem₂ : l₂.flip.var ∈ clause.vars (l₁ :: l₂ :: ls),
-  { simp [flip_var_eq, clause.vars] },
-  have hnmem₁ : g.fresh.1 ∉ clause.vars (l₁ :: l₂ :: ls),
-  { have := set.disjoint_left.mp hdis (fresh_mem_stock g),
-    assumption }, -- TODO coercion is silly
-  have hnmem₂ : g.fresh.2.fresh.1 ∉ clause.vars (l₁ :: l₂ :: ls),
-  { have := fresh_mem_stock g.fresh.2,
-    have := set.disjoint_left.mp hdis (fresh_stock_subset g this),
-    assumption }, -- TODO this too
-  cases ls with l₃ ls,
-  { sorry }, /-split,
-    { intro heval,
-      rw ← amo.eval at heval,
-      cases h₁ : (literal.eval τ l₁),
-      { use assignment.ite (clause.vars [l₁, l₂]) τ all_ff,
-        split,
-        { rw eval_tt_iff_forall_clause_eval_tt,
-          intros c hc,
-          simp [sinz] at hc,
-          rw eval_tt_iff_exists_literal_eval_tt,
-          rcases hc with (rfl | rfl | rfl),
-          { use l₁.flip,
-            rw [ite_pos_lit hmem₁, eval_flip],
-            simp [h₁] },
-          { use Neg g.fresh.1,
-            simp [literal.eval, ite_neg hnmem₁, all_ff] },
-          { use Neg g.fresh.1,
-            simp [literal.eval, ite_neg hnmem₁, all_ff] } },
-        { exact (ite_eqod (clause.vars [l₁, l₂]) τ _).symm } },
-      { use assignment.ite (clause.vars [l₁, l₂]) τ all_tt,
-        split,
-        { rw eval_tt_iff_forall_clause_eval_tt,
-          intros c hc,
-          simp [sinz] at hc,
-          rw eval_tt_iff_exists_literal_eval_tt,
-          rcases hc with (rfl | rfl | rfl),
-          { use Pos g.fresh.1,
-            simp [literal.eval, ite_neg hnmem₁, all_tt] },
-          { use Pos g.fresh.2.fresh.1,
-            simp [literal.eval, ite_neg hnmem₂, all_tt] },
-          { use l₂.flip,
-            have := amo.amo_eval_tt_iff_distinct_eval_ff_of_eval_tt.mp heval,
-            have := this (distinct_double l₁ l₂) h₁,
-            simp [ite_pos_lit hmem₂],
-            rw eval_flip,
-            simp [this] } },
-        { exact (ite_eqod (clause.vars [l₁, l₂]) τ _).symm } } },
-    { rintros ⟨σ, heval, hs⟩,
-    have heq : literal.eval τ l₂ = literal.eval σ l₂,
-    { have : l₂.var ∈ clause.vars [l₁, l₂],
-      { simp [clause.vars] },
-        exact eval_eq_of_eqod_of_var_mem hs this },
-      rw [← amo.eval, eval_eq_amo_of_eqod hs],
-      rw eval_tt_iff_forall_clause_eval_tt at heval,
-      cases h₁ : (literal.eval σ l₁),
-      { rw [eval_cons_neg h₁, amo.eval_singleton] },
-      { have : ∀ (lit₁ lit₂ : literal V), (distinct lit₁ lit₂ [l₁, l₂]) → 
-          lit₁.eval τ = tt → lit₂.eval τ = ff,
-        { intros lit₁ lit₂ hd _,
-          rcases eq_of_distinct_double hd with ⟨rfl, rfl⟩,
-          simp [sinz, clause.eval, eval_flip, literal.eval, h₁] at heval,
-          rcases heval with ⟨hs₁, hs₂, hs₃⟩,
-          simp [hs₁] at hs₃,
-          rw heq,
-          exact hs₃ },
-        rw ← eval_eq_amo_of_eqod hs,
-        exact amo_eval_tt_iff_distinct_eval_ff_of_eval_tt.mpr this } } }, -/
-  { split,
-    { intro heval,
-      rw ← amo.eval at heval,
-      have hless : length (l₂ :: l₃ :: ls) < length (l₁ :: l₂ :: l₃ :: ls), simp,
-      have hlen : length (l₂ :: l₃ :: ls) ≥ 2, dec_trivial,
-      have ihred := ih _ hless hlen hdis',
-      cases h₁ : (literal.eval τ l₁),
-      { sorry }, /- rw eval_cons_neg h₁ at heval,
-        rcases ihred.mp heval with ⟨σ, heval', hs⟩,
-        use assignment.ite (cnf.vars (sinz (l₂ :: l₃ :: ls) g.fresh.2 hdis')) σ 
-            (assignment.ite {l₁.var} τ all_ff),
-        have heval₁ : literal.eval (assignment.ite (cnf.vars (sinz (l₂ :: l₃ :: ls) g.fresh.2 hdis')) σ 
-            (assignment.ite {l₁.var} τ all_ff)) l₁ = ff,
-        { sorry },
-        have heval₂ : (assignment.ite (cnf.vars (sinz (l₂ :: l₃ :: ls) g.fresh.2 hdis')) σ 
-            (assignment.ite {l₁.var} τ all_ff)) g.fresh.1 = ff,
-        { sorry },
-        split,
-        { rw [eval_tt_iff_forall_clause_eval_tt, sinz],
-          intros c hc,
-          rw eval_tt_iff_exists_literal_eval_tt,
-          simp at hc,
-          rcases hc with (rfl | rfl | rfl | hc),
-          { use l₁.flip,
-            simp [eval_flip, heval₁] },
-          { use Neg g.fresh.1,
-            simp [literal.eval, heval₂] },
-          { use Neg g.fresh.1,
-            simp [literal.eval, heval₂] },
-          { rw ← eval_tt_iff_exists_literal_eval_tt,
-            rw eval_tt_iff_forall_clause_eval_tt at heval',
-            rw ← heval' c hc,
-            apply eval_eq_clause_of_eqod,
-            apply eqod_subset (clause_vars_subset_of_vars_of_mem hc),
-            intros v hv,
-            rw ite_pos hv } },
-        { intros v hv,
-          rcases finset.mem_union.mp hv with (hvmem | hvmem),
-          { cases l₁;
-            { simp [literal.flip, literal.eval, var] at h₁ hvmem heval₁ |-,
-              simp [heval₁, hvmem, h₁] } },
-          { rw ite_pos (mem_sinz_vars_of_mem hdis' hlen hvmem),
-            exact hs v hvmem }
-        } }, -/
-      { sorry } },
-      /-
-      { rw eval_cons_pos h₁ at heval,
-        rw amz.eval_tt_iff_forall_eval_ff at heval,
-        use assignment.ite (clause.vars (l₁ :: l₂ :: l₃ :: ls)) τ all_tt,
-        have heval₁ : literal.eval (assignment.ite (clause.vars (l₁ :: l₂ :: l₃ :: ls)) τ all_tt) l₁ = tt,
-        { sorry },
-        have heval₂ : (assignment.ite (clause.vars (l₁ :: l₂ :: l₃ :: ls)) τ all_tt) g.fresh.1 = tt,
-        { sorry },
-        have heval₃ : (assignment.ite (clause.vars (l₁ :: l₂ :: l₃ :: ls)) τ all_tt) g.fresh.2.fresh.1 = tt,
-        { sorry },
-        split,
-        { rw [eval_tt_iff_forall_clause_eval_tt, sinz],
-          intros c hc,
-          simp at hc,
-          rw eval_tt_iff_exists_literal_eval_tt,
-          rcases hc with (rfl | rfl | rfl | hc),
-          { use Pos g.fresh.1,
-            simp [literal.eval, heval₂] },
-          { use Pos g.fresh.2.fresh.1,
-            simp [literal.eval, heval₃] },
-          { use l₂.flip,
-            rw [ite_pos_lit hmem₂, eval_flip],
-            simp [ite_pos_lit hmem₂, eval_flip, heval l₂ (mem_cons_self l₂ _)] },
-          { rw ← amz.eval_tt_iff_forall_eval_ff at heval,
-            have := all_tt_eval_tt_of_amz_eval_tt hdis' hlen heval,
-            rw eval_tt_iff_forall_clause_eval_tt at this,
-            have := this c hc,
-            rcases eval_tt_iff_exists_literal_eval_tt.mp this with ⟨l, hlmem, hle⟩,
-            use [l, hlmem],
-            by_cases hlin : l.var ∈ clause.vars (l₂ :: l₃ :: ls),
-            { rw ite_pos_lit hlin at hle,
-              rw ite_pos_lit (vars_subset_of_vars_cons l₁ (l₂ :: l₃ :: ls) hlin),
-              exact hle },
-            { rw ite_neg_lit hlin at hle,
-              -- show l.var is not equal to l₁.var
-              sorry } } },
-        { intros v hv, rw ite_pos hv } } }, -/
-    {
-      rintros ⟨σ, heval, heqod⟩,
-      rw [sinz, eval_tt_iff_forall_clause_eval_tt] at heval,
-      simp at heval,
-    }
-  }
 end
 -/
 
